Updated examples.

tests/AddDelay_noinfer.bpl
@@ -11,7 +11,7 @@ var M: MType;
 var C: CType;
 var R: CType;
 var I: CType;
-var St: [Actor]State;
+var T: CType;
 
 const unique this#: Actor;
 type List a = [int]a;
@@ -24,7 +24,7 @@ function AT#Min(x:int, y: int): int { if x <= y then x else y }
 // ---------------------------------------------------------------
 
 procedure Add#init#0()
-  modifies C, R, M, I, St;
+  modifies C, R, M, I;
 {
   var in1: Chan (int);
   var in2: Chan (int);
@@ -39,7 +39,7 @@ procedure Add#init#0()
   );
 }
 procedure Add#anon$0#1()
-  modifies C, R, M, I, St;
+  modifies C, R, M, I;
 {
   var in1: Chan (int);
   var in2: Chan (int);
@@ -58,7 +58,6 @@ procedure Add#anon$0#1()
   R[in1] := R[in1] + 1;
   in2#0 := M[in2][R[in2]];
   R[in2] := R[in2] + 1;
-  assume true;
   M[out][C[out]] := in1#0 + in2#0;
   C[out] := C[out] + 1;
   assert {:msg "3.20: Action at 5.3 might not preserve invariant (#2)"} (R[in1] == C[out]) && (R[in2] == C[out]);
@@ -67,7 +66,7 @@ procedure Add#anon$0#1()
   );
 }
 procedure Delay#init#2()
-  modifies C, R, M, I, St;
+  modifies C, R, M, I;
 {
   var in: Chan (int);
   var out: Chan (int);
@@ -75,7 +74,6 @@ procedure Delay#init#2()
   assume in != out;
   assume R[in] == 0;
   assume C[out] == 0;
-  assume true;
   M[out][C[out]] := k;
   C[out] := C[out] + 1;
   assert {:msg "10.20: Initialization might not establish the invariant (#4)"} R[in] == (C[out] - 1);
@@ -85,7 +83,7 @@ procedure Delay#init#2()
   );
 }
 procedure Delay#anon$2#3()
-  modifies C, R, M, I, St;
+  modifies C, R, M, I;
 {
   var in: Chan (int);
   var out: Chan (int);
@@ -101,7 +99,6 @@ procedure Delay#anon$2#3()
   );
   in#0 := M[in][R[in]];
   R[in] := R[in] + 1;
-  assume true;
   M[out][C[out]] := in#0;
   C[out] := C[out] + 1;
   assert {:msg "10.20: Action at 14.3 might not preserve invariant (#7)"} R[in] == (C[out] - 1);
@@ -111,7 +108,7 @@ procedure Delay#anon$2#3()
   );
 }
 procedure Split#init#4()
-  modifies C, R, M, I, St;
+  modifies C, R, M, I;
 {
   var in: Chan (int);
   var out1: Chan (int);
@@ -126,7 +123,7 @@ procedure Split#init#4()
   );
 }
 procedure Split#anon$3#5()
-  modifies C, R, M, I, St;
+  modifies C, R, M, I;
 {
   var in: Chan (int);
   var out1: Chan (int);
@@ -142,7 +139,6 @@ procedure Split#anon$3#5()
   );
   in#0 := M[in][R[in]];
   R[in] := R[in] + 1;
-  assume true;
   M[out1][C[out1]] := in#0;
   C[out1] := C[out1] + 1;
   M[out2][C[out2]] := in#0;
@@ -153,7 +149,7 @@ procedure Split#anon$3#5()
   );
 }
 procedure Net#init#6()
-  modifies C, R, M, I, St;
+  modifies C, R, M, I;
 {
   var Net#add: Actor;
   var Net#del: Actor;
@@ -191,38 +187,24 @@ procedure Net#init#6()
   assume R[Net#d] == 0;
   assume C[Net#e] == 0;
   assume R[Net#e] == 0;
-  assume (R[Net#a] == C[Net#c]) && (R[Net#b] == C[Net#c]);
-  assume (forall i: int :: 
-    (0 <= i) && (i < C[Net#c]) ==> (M[Net#c][i] == (M[Net#a][i] + M[Net#b][i]))
-  );
   assume 0 == 0;
   M[Net#b][C[Net#b]] := 0;
   C[Net#b] := C[Net#b] + 1;
-  assume R[Net#e] == (C[Net#b] - 1);
-  assume M[Net#b][0] == 0;
-  assume (forall i: int :: 
-    ((0 + 1) <= i) && (i < (C[Net#b] - 0)) ==> (M[Net#b][i] == M[Net#e][i - 1])
-  );
-  assume (R[Net#c] == C[Net#d]) && (R[Net#c] == C[Net#e]);
-  assume (forall i: int :: 
-    (0 <= i) && (i < C[Net#d]) ==> (M[Net#d][i] == M[Net#c][i]) && (M[Net#e][i] == M[Net#c][i])
-  );
-  assert {:msg "34.15: Initialization of network 'Net' might not establish the channel invariant (#14)"} (I[Net#a] == I[Net#b]) && (I[Net#b] == I[Net#c]) && (I[Net#c] == I[Net#d]) && (I[Net#d] == I[Net#e]);
-  assert {:msg "35.15: Initialization of network 'Net' might not establish the channel invariant (#15)"} (I[Net#c] > 0) ==> (M[Net#c][0] == M[Net#a][0]);
-  assert {:msg "36.15: Initialization of network 'Net' might not establish the channel invariant (#16)"} (I[Net#c] > 0) ==> (M[Net#c][I[Net#c] - 1] == M[Net#b][I[Net#b]]);
-  assert {:msg "Initialization of network 'Net' might not establish the channel invariant (#17)"} true && (forall idx$: int :: 
-    (I[Net#a] <= idx$) && (idx$ < C[Net#a]) ==> (0 <= M[Net#a][idx$])
-  );
+  assert {:msg "34.15: Initialization of network 'Net' might not establish the channel invariant (#14)"} I[Net#a] == I[Net#b];
+  assert {:msg "35.15: Initialization of network 'Net' might not establish the channel invariant (#15)"} I[Net#b] == I[Net#c];
+  assert {:msg "36.15: Initialization of network 'Net' might not establish the channel invariant (#16)"} I[Net#c] == I[Net#d];
+  assert {:msg "37.15: Initialization of network 'Net' might not establish the channel invariant (#17)"} I[Net#d] == I[Net#e];
+  assert {:msg "38.15: Initialization of network 'Net' might not establish the channel invariant (#18)"} (I[Net#c] > 0) ==> (M[Net#c][0] == M[Net#a][0]);
+  assert {:msg "39.15: Initialization of network 'Net' might not establish the channel invariant (#19)"} (I[Net#c] > 0) ==> (M[Net#c][I[Net#c] - 1] == M[Net#b][I[Net#b]]);
   I := R;
-  C[Net#b] := C[Net#b] - 1;
-  assert {:msg "45.5: The initialization might produce unspecified tokens on channel a (#18)"} (C[Net#a] - R[Net#a]) == 0;
-  assert {:msg "46.5: The initialization might produce unspecified tokens on channel b (#19)"} (C[Net#b] - R[Net#b]) == 0;
-  assert {:msg "47.5: The initialization might produce unspecified tokens on channel c (#20)"} (C[Net#c] - R[Net#c]) == 0;
-  assert {:msg "48.5: The initialization might produce unspecified tokens on channel d (#21)"} (C[Net#d] - R[Net#d]) == 0;
-  assert {:msg "49.5: The initialization might produce unspecified tokens on channel e (#22)"} (C[Net#e] - R[Net#e]) == 0;
+  assert {:msg "32.13: Network initialization might not establish the network invariant (#20)"} (C[Net#b] - R[Net#b]) == 1;
+  assert {:msg "48.5: The initialization might produce unspecified tokens on channel a (#21)"} (C[Net#a] - R[Net#a]) == 0;
+  assert {:msg "50.5: The initialization might produce unspecified tokens on channel c (#22)"} (C[Net#c] - R[Net#c]) == 0;
+  assert {:msg "51.5: The initialization might produce unspecified tokens on channel d (#23)"} (C[Net#d] - R[Net#d]) == 0;
+  assert {:msg "52.5: The initialization might produce unspecified tokens on channel e (#24)"} (C[Net#e] - R[Net#e]) == 0;
 }
 procedure Net##Add#anon$0#7()
-  modifies C, R, M, I, St;
+  modifies C, R, M, I;
 {
   var Net#add: Actor;
   var Net#del: Actor;
@@ -252,13 +234,15 @@ procedure Net##Add#anon$0#7()
   assume 0 <= I[Net#e];
   assume I[Net#e] <= R[Net#e];
   assume R[Net#e] <= C[Net#e];
-  assume (I[Net#a] == I[Net#b]) && (I[Net#b] == I[Net#c]) && (I[Net#c] == I[Net#d]) && (I[Net#d] == I[Net#e]);
+  assume I[Net#a] == I[Net#b];
+  assume I[Net#b] == I[Net#c];
+  assume I[Net#c] == I[Net#d];
+  assume I[Net#d] == I[Net#e];
   assume (I[Net#c] > 0) ==> (M[Net#c][0] == M[Net#a][0]);
   assume (I[Net#c] > 0) ==> (M[Net#c][I[Net#c] - 1] == M[Net#b][I[Net#b]]);
-  assume true && (forall idx$: int :: 
-    (I[Net#a] <= idx$) && (idx$ < C[Net#a]) ==> (0 <= M[Net#a][idx$])
-  );
-  assume (R[Net#a] == C[Net#c]) && (R[Net#b] == C[Net#c]);
+  assume 0 <= M[Net#a][I[Net#a]];
+  assume R[Net#a] == C[Net#c];
+  assume R[Net#b] == C[Net#c];
   assume (forall i: int :: 
     (0 <= i) && (i < C[Net#c]) ==> (M[Net#c][i] == (M[Net#a][i] + M[Net#b][i]))
   );
@@ -267,34 +251,42 @@ procedure Net##Add#anon$0#7()
   assume (forall i: int :: 
     ((0 + 1) <= i) && (i < (C[Net#b] - 0)) ==> (M[Net#b][i] == M[Net#e][i - 1])
   );
-  assume (R[Net#c] == C[Net#d]) && (R[Net#c] == C[Net#e]);
+  assume R[Net#c] == C[Net#d];
+  assume R[Net#c] == C[Net#e];
   assume (forall i: int :: 
     (0 <= i) && (i < C[Net#d]) ==> (M[Net#d][i] == M[Net#c][i]) && (M[Net#e][i] == M[Net#c][i])
   );
   assume (1 <= (C[Net#a] - R[Net#a])) && (1 <= (C[Net#b] - R[Net#b]));
-  assume (R[Net#a] == C[Net#c]) && (R[Net#b] == C[Net#c]);
-  assume (forall i: int :: 
-    (0 <= in1#i) && (in1#i < C[Net#c]) ==> (M[Net#c][in1#i] == (M[Net#a][in1#i] + M[Net#b][in1#i]))
-  );
   in1#i := M[Net#a][R[Net#a]];
   R[Net#a] := R[Net#a] + 1;
   in2#j := M[Net#b][R[Net#b]];
   R[Net#b] := R[Net#b] + 1;
   M[Net#c][C[Net#c]] := in1#i + in2#j;
   C[Net#c] := C[Net#c] + 1;
-  assume (R[Net#a] == C[Net#c]) && (R[Net#b] == C[Net#c]);
+  assume R[Net#a] == C[Net#c];
+  assume R[Net#b] == C[Net#c];
   assume (forall i: int :: 
-    (0 <= in1#i) && (in1#i < C[Net#c]) ==> (M[Net#c][in1#i] == (M[Net#a][in1#i] + M[Net#b][in1#i]))
+    (0 <= i) && (i < C[Net#c]) ==> (M[Net#c][i] == (M[Net#a][i] + M[Net#b][i]))
   );
-  assert {:msg "34.15: Action at 5.3 ('anon$0') for actor instance 'add' might not preserve the channel invariant (#23)"} (I[Net#a] == I[Net#b]) && (I[Net#b] == I[Net#c]) && (I[Net#c] == I[Net#d]) && (I[Net#d] == I[Net#e]);
-  assert {:msg "35.15: Action at 5.3 ('anon$0') for actor instance 'add' might not preserve the channel invariant (#24)"} (I[Net#c] > 0) ==> (M[Net#c][0] == M[Net#a][0]);
-  assert {:msg "36.15: Action at 5.3 ('anon$0') for actor instance 'add' might not preserve the channel invariant (#25)"} (I[Net#c] > 0) ==> (M[Net#c][I[Net#c] - 1] == M[Net#b][I[Net#b]]);
-  assert {:msg "Action at 5.3 ('anon$0') for actor instance 'add' might not preserve the channel invariant (#26)"} true && (forall idx$: int :: 
-    (I[Net#a] <= idx$) && (idx$ < C[Net#a]) ==> (0 <= M[Net#a][idx$])
+  assume R[Net#e] == (C[Net#b] - 1);
+  assume M[Net#b][0] == 0;
+  assume (forall i: int :: 
+    ((0 + 1) <= i) && (i < (C[Net#b] - 0)) ==> (M[Net#b][i] == M[Net#e][i - 1])
   );
+  assume R[Net#c] == C[Net#d];
+  assume R[Net#c] == C[Net#e];
+  assume (forall i: int :: 
+    (0 <= i) && (i < C[Net#d]) ==> (M[Net#d][i] == M[Net#c][i]) && (M[Net#e][i] == M[Net#c][i])
+  );
+  assert {:msg "34.15: Action at 5.3 ('anon$0') for actor instance 'add' might not preserve the channel invariant (#25)"} I[Net#a] == I[Net#b];
+  assert {:msg "35.15: Action at 5.3 ('anon$0') for actor instance 'add' might not preserve the channel invariant (#26)"} I[Net#b] == I[Net#c];
+  assert {:msg "36.15: Action at 5.3 ('anon$0') for actor instance 'add' might not preserve the channel invariant (#27)"} I[Net#c] == I[Net#d];
+  assert {:msg "37.15: Action at 5.3 ('anon$0') for actor instance 'add' might not preserve the channel invariant (#28)"} I[Net#d] == I[Net#e];
+  assert {:msg "38.15: Action at 5.3 ('anon$0') for actor instance 'add' might not preserve the channel invariant (#29)"} (I[Net#c] > 0) ==> (M[Net#c][0] == M[Net#a][0]);
+  assert {:msg "39.15: Action at 5.3 ('anon$0') for actor instance 'add' might not preserve the channel invariant (#30)"} (I[Net#c] > 0) ==> (M[Net#c][I[Net#c] - 1] == M[Net#b][I[Net#b]]);
 }
 procedure Net##Delay#anon$2#8()
-  modifies C, R, M, I, St;
+  modifies C, R, M, I;
 {
   var Net#add: Actor;
   var Net#del: Actor;
@@ -323,13 +315,15 @@ procedure Net##Delay#anon$2#8()
   assume 0 <= I[Net#e];
   assume I[Net#e] <= R[Net#e];
   assume R[Net#e] <= C[Net#e];
-  assume (I[Net#a] == I[Net#b]) && (I[Net#b] == I[Net#c]) && (I[Net#c] == I[Net#d]) && (I[Net#d] == I[Net#e]);
+  assume I[Net#a] == I[Net#b];
+  assume I[Net#b] == I[Net#c];
+  assume I[Net#c] == I[Net#d];
+  assume I[Net#d] == I[Net#e];
   assume (I[Net#c] > 0) ==> (M[Net#c][0] == M[Net#a][0]);
   assume (I[Net#c] > 0) ==> (M[Net#c][I[Net#c] - 1] == M[Net#b][I[Net#b]]);
-  assume true && (forall idx$: int :: 
-    (I[Net#a] <= idx$) && (idx$ < C[Net#a]) ==> (0 <= M[Net#a][idx$])
-  );
-  assume (R[Net#a] == C[Net#c]) && (R[Net#b] == C[Net#c]);
+  assume 0 <= M[Net#a][I[Net#a]];
+  assume R[Net#a] == C[Net#c];
+  assume R[Net#b] == C[Net#c];
   assume (forall i: int :: 
     (0 <= i) && (i < C[Net#c]) ==> (M[Net#c][i] == (M[Net#a][i] + M[Net#b][i]))
   );
@@ -338,34 +332,40 @@ procedure Net##Delay#anon$2#8()
   assume (forall i: int :: 
     ((0 + 1) <= i) && (i < (C[Net#b] - 0)) ==> (M[Net#b][i] == M[Net#e][i - 1])
   );
-  assume (R[Net#c] == C[Net#d]) && (R[Net#c] == C[Net#e]);
+  assume R[Net#c] == C[Net#d];
+  assume R[Net#c] == C[Net#e];
   assume (forall i: int :: 
     (0 <= i) && (i < C[Net#d]) ==> (M[Net#d][i] == M[Net#c][i]) && (M[Net#e][i] == M[Net#c][i])
   );
   assume 1 <= (C[Net#e] - R[Net#e]);
-  assume R[Net#e] == (C[Net#b] - 1);
-  assume M[Net#b][0] == 0;
-  assume (forall i: int :: 
-    ((0 + 1) <= in#i) && (in#i < (C[Net#b] - 0)) ==> (M[Net#b][in#i] == M[Net#e][in#i - 1])
-  );
   in#i := M[Net#e][R[Net#e]];
   R[Net#e] := R[Net#e] + 1;
   M[Net#b][C[Net#b]] := in#i;
   C[Net#b] := C[Net#b] + 1;
+  assume R[Net#a] == C[Net#c];
+  assume R[Net#b] == C[Net#c];
+  assume (forall i: int :: 
+    (0 <= i) && (i < C[Net#c]) ==> (M[Net#c][i] == (M[Net#a][i] + M[Net#b][i]))
+  );
   assume R[Net#e] == (C[Net#b] - 1);
   assume M[Net#b][0] == 0;
   assume (forall i: int :: 
-    ((0 + 1) <= in#i) && (in#i < (C[Net#b] - 0)) ==> (M[Net#b][in#i] == M[Net#e][in#i - 1])
+    ((0 + 1) <= i) && (i < (C[Net#b] - 0)) ==> (M[Net#b][i] == M[Net#e][i - 1])
   );
-  assert {:msg "34.15: Action at 14.3 ('anon$2') for actor instance 'del' might not preserve the channel invariant (#27)"} (I[Net#a] == I[Net#b]) && (I[Net#b] == I[Net#c]) && (I[Net#c] == I[Net#d]) && (I[Net#d] == I[Net#e]);
-  assert {:msg "35.15: Action at 14.3 ('anon$2') for actor instance 'del' might not preserve the channel invariant (#28)"} (I[Net#c] > 0) ==> (M[Net#c][0] == M[Net#a][0]);
-  assert {:msg "36.15: Action at 14.3 ('anon$2') for actor instance 'del' might not preserve the channel invariant (#29)"} (I[Net#c] > 0) ==> (M[Net#c][I[Net#c] - 1] == M[Net#b][I[Net#b]]);
-  assert {:msg "Action at 14.3 ('anon$2') for actor instance 'del' might not preserve the channel invariant (#30)"} true && (forall idx$: int :: 
-    (I[Net#a] <= idx$) && (idx$ < C[Net#a]) ==> (0 <= M[Net#a][idx$])
+  assume R[Net#c] == C[Net#d];
+  assume R[Net#c] == C[Net#e];
+  assume (forall i: int :: 
+    (0 <= i) && (i < C[Net#d]) ==> (M[Net#d][i] == M[Net#c][i]) && (M[Net#e][i] == M[Net#c][i])
   );
+  assert {:msg "34.15: Action at 14.3 ('anon$2') for actor instance 'del' might not preserve the channel invariant (#31)"} I[Net#a] == I[Net#b];
+  assert {:msg "35.15: Action at 14.3 ('anon$2') for actor instance 'del' might not preserve the channel invariant (#32)"} I[Net#b] == I[Net#c];
+  assert {:msg "36.15: Action at 14.3 ('anon$2') for actor instance 'del' might not preserve the channel invariant (#33)"} I[Net#c] == I[Net#d];
+  assert {:msg "37.15: Action at 14.3 ('anon$2') for actor instance 'del' might not preserve the channel invariant (#34)"} I[Net#d] == I[Net#e];
+  assert {:msg "38.15: Action at 14.3 ('anon$2') for actor instance 'del' might not preserve the channel invariant (#35)"} (I[Net#c] > 0) ==> (M[Net#c][0] == M[Net#a][0]);
+  assert {:msg "39.15: Action at 14.3 ('anon$2') for actor instance 'del' might not preserve the channel invariant (#36)"} (I[Net#c] > 0) ==> (M[Net#c][I[Net#c] - 1] == M[Net#b][I[Net#b]]);
 }
 procedure Net##Split#anon$3#9()
-  modifies C, R, M, I, St;
+  modifies C, R, M, I;
 {
   var Net#add: Actor;
   var Net#del: Actor;
@@ -394,13 +394,15 @@ procedure Net##Split#anon$3#9()
   assume 0 <= I[Net#e];
   assume I[Net#e] <= R[Net#e];
   assume R[Net#e] <= C[Net#e];
-  assume (I[Net#a] == I[Net#b]) && (I[Net#b] == I[Net#c]) && (I[Net#c] == I[Net#d]) && (I[Net#d] == I[Net#e]);
+  assume I[Net#a] == I[Net#b];
+  assume I[Net#b] == I[Net#c];
+  assume I[Net#c] == I[Net#d];
+  assume I[Net#d] == I[Net#e];
   assume (I[Net#c] > 0) ==> (M[Net#c][0] == M[Net#a][0]);
   assume (I[Net#c] > 0) ==> (M[Net#c][I[Net#c] - 1] == M[Net#b][I[Net#b]]);
-  assume true && (forall idx$: int :: 
-    (I[Net#a] <= idx$) && (idx$ < C[Net#a]) ==> (0 <= M[Net#a][idx$])
-  );
-  assume (R[Net#a] == C[Net#c]) && (R[Net#b] == C[Net#c]);
+  assume 0 <= M[Net#a][I[Net#a]];
+  assume R[Net#a] == C[Net#c];
+  assume R[Net#b] == C[Net#c];
   assume (forall i: int :: 
     (0 <= i) && (i < C[Net#c]) ==> (M[Net#c][i] == (M[Net#a][i] + M[Net#b][i]))
   );
@@ -409,74 +411,20 @@ procedure Net##Split#anon$3#9()
   assume (forall i: int :: 
     ((0 + 1) <= i) && (i < (C[Net#b] - 0)) ==> (M[Net#b][i] == M[Net#e][i - 1])
   );
-  assume (R[Net#c] == C[Net#d]) && (R[Net#c] == C[Net#e]);
+  assume R[Net#c] == C[Net#d];
+  assume R[Net#c] == C[Net#e];
   assume (forall i: int :: 
     (0 <= i) && (i < C[Net#d]) ==> (M[Net#d][i] == M[Net#c][i]) && (M[Net#e][i] == M[Net#c][i])
   );
   assume 1 <= (C[Net#c] - R[Net#c]);
-  assume (R[Net#c] == C[Net#d]) && (R[Net#c] == C[Net#e]);
-  assume (forall i: int :: 
-    (0 <= in#i) && (in#i < C[Net#d]) ==> (M[Net#d][in#i] == M[Net#c][in#i]) && (M[Net#e][in#i] == M[Net#c][in#i])
-  );
   in#i := M[Net#c][R[Net#c]];
   R[Net#c] := R[Net#c] + 1;
   M[Net#d][C[Net#d]] := in#i;
   C[Net#d] := C[Net#d] + 1;
   M[Net#e][C[Net#e]] := in#i;
   C[Net#e] := C[Net#e] + 1;
-  assume (R[Net#c] == C[Net#d]) && (R[Net#c] == C[Net#e]);
-  assume (forall i: int :: 
-    (0 <= in#i) && (in#i < C[Net#d]) ==> (M[Net#d][in#i] == M[Net#c][in#i]) && (M[Net#e][in#i] == M[Net#c][in#i])
-  );
-  assert {:msg "34.15: Action at 21.3 ('anon$3') for actor instance 'spl' might not preserve the channel invariant (#31)"} (I[Net#a] == I[Net#b]) && (I[Net#b] == I[Net#c]) && (I[Net#c] == I[Net#d]) && (I[Net#d] == I[Net#e]);
-  assert {:msg "35.15: Action at 21.3 ('anon$3') for actor instance 'spl' might not preserve the channel invariant (#32)"} (I[Net#c] > 0) ==> (M[Net#c][0] == M[Net#a][0]);
-  assert {:msg "36.15: Action at 21.3 ('anon$3') for actor instance 'spl' might not preserve the channel invariant (#33)"} (I[Net#c] > 0) ==> (M[Net#c][I[Net#c] - 1] == M[Net#b][I[Net#b]]);
-  assert {:msg "Action at 21.3 ('anon$3') for actor instance 'spl' might not preserve the channel invariant (#34)"} true && (forall idx$: int :: 
-    (I[Net#a] <= idx$) && (idx$ < C[Net#a]) ==> (0 <= M[Net#a][idx$])
-  );
-}
-procedure Net#entry()
-  modifies C, R, M, I, St;
-{
-  var Net#add: Actor;
-  var Net#del: Actor;
-  var Net#spl: Actor;
-  var Net#a: Chan (int);
-  var Net#b: Chan (int);
-  var Net#c: Chan (int);
-  var Net#d: Chan (int);
-  var Net#e: Chan (int);
-  assume (Net#add != Net#del) && (Net#add != Net#spl) && (Net#del != Net#spl);
-  assume (Net#a != Net#b) && (Net#a != Net#c) && (Net#a != Net#d) && (Net#a != Net#e) && (Net#b != Net#c) && (Net#b != Net#d) && (Net#b != Net#e) && (Net#c != Net#d) && (Net#c != Net#e) && (Net#d != Net#e);
-  assume 0 <= I[Net#a];
-  assume I[Net#a] <= R[Net#a];
-  assume R[Net#a] <= C[Net#a];
-  assume 0 <= I[Net#b];
-  assume I[Net#b] <= R[Net#b];
-  assume R[Net#b] <= C[Net#b];
-  assume 0 <= I[Net#c];
-  assume I[Net#c] <= R[Net#c];
-  assume R[Net#c] <= C[Net#c];
-  assume 0 <= I[Net#d];
-  assume I[Net#d] <= R[Net#d];
-  assume R[Net#d] <= C[Net#d];
-  assume I[Net#d] == R[Net#d];
-  assume 0 <= I[Net#e];
-  assume I[Net#e] <= R[Net#e];
-  assume R[Net#e] <= C[Net#e];
-  assume C[Net#a] == R[Net#a];
-  assume C[Net#b] == R[Net#b];
-  assume C[Net#c] == R[Net#c];
-  assume C[Net#d] == R[Net#d];
-  assume C[Net#e] == R[Net#e];
-  C[Net#b] := C[Net#b] + 1;
-  assume (I[Net#a] == I[Net#b]) && (I[Net#b] == I[Net#c]) && (I[Net#c] == I[Net#d]) && (I[Net#d] == I[Net#e]);
-  assume (I[Net#c] > 0) ==> (M[Net#c][0] == M[Net#a][0]);
-  assume (I[Net#c] > 0) ==> (M[Net#c][I[Net#c] - 1] == M[Net#b][I[Net#b]]);
-  assume true && (forall idx$: int :: 
-    (I[Net#a] <= idx$) && (idx$ < C[Net#a]) ==> (0 <= M[Net#a][idx$])
-  );
-  assume (R[Net#a] == C[Net#c]) && (R[Net#b] == C[Net#c]);
+  assume R[Net#a] == C[Net#c];
+  assume R[Net#b] == C[Net#c];
   assume (forall i: int :: 
     (0 <= i) && (i < C[Net#c]) ==> (M[Net#c][i] == (M[Net#a][i] + M[Net#b][i]))
   );
@@ -485,16 +433,20 @@ procedure Net#entry()
   assume (forall i: int :: 
     ((0 + 1) <= i) && (i < (C[Net#b] - 0)) ==> (M[Net#b][i] == M[Net#e][i - 1])
   );
-  assume (R[Net#c] == C[Net#d]) && (R[Net#c] == C[Net#e]);
+  assume R[Net#c] == C[Net#d];
+  assume R[Net#c] == C[Net#e];
   assume (forall i: int :: 
     (0 <= i) && (i < C[Net#d]) ==> (M[Net#d][i] == M[Net#c][i]) && (M[Net#e][i] == M[Net#c][i])
   );
-  assert {:msg "24.1: Sub-actors in the network might fire without network input. This is not permitted. (#35)"} !((1 <= (C[Net#a] - R[Net#a])) && (1 <= (C[Net#b] - R[Net#b])));
-  assert {:msg "24.1: Sub-actors in the network might fire without network input. This is not permitted. (#36)"} !(1 <= (C[Net#e] - R[Net#e]));
-  assert {:msg "24.1: Sub-actors in the network might fire without network input. This is not permitted. (#37)"} !(1 <= (C[Net#c] - R[Net#c]));
+  assert {:msg "34.15: Action at 21.3 ('anon$3') for actor instance 'spl' might not preserve the channel invariant (#37)"} I[Net#a] == I[Net#b];
+  assert {:msg "35.15: Action at 21.3 ('anon$3') for actor instance 'spl' might not preserve the channel invariant (#38)"} I[Net#b] == I[Net#c];
+  assert {:msg "36.15: Action at 21.3 ('anon$3') for actor instance 'spl' might not preserve the channel invariant (#39)"} I[Net#c] == I[Net#d];
+  assert {:msg "37.15: Action at 21.3 ('anon$3') for actor instance 'spl' might not preserve the channel invariant (#40)"} I[Net#d] == I[Net#e];
+  assert {:msg "38.15: Action at 21.3 ('anon$3') for actor instance 'spl' might not preserve the channel invariant (#41)"} (I[Net#c] > 0) ==> (M[Net#c][0] == M[Net#a][0]);
+  assert {:msg "39.15: Action at 21.3 ('anon$3') for actor instance 'spl' might not preserve the channel invariant (#42)"} (I[Net#c] > 0) ==> (M[Net#c][I[Net#c] - 1] == M[Net#b][I[Net#b]]);
 }
 procedure Net#anon$4#input#in#10()
-  modifies C, R, M, I, St;
+  modifies C, R, M, I;
 {
   var Net#add: Actor;
   var Net#del: Actor;
@@ -522,14 +474,16 @@ procedure Net#anon$4#input#in#10()
   assume 0 <= I[Net#e];
   assume I[Net#e] <= R[Net#e];
   assume R[Net#e] <= C[Net#e];
-  assume C[Net#a] < 1;
-  assume (I[Net#a] == I[Net#b]) && (I[Net#b] == I[Net#c]) && (I[Net#c] == I[Net#d]) && (I[Net#d] == I[Net#e]);
+  assume (C[Net#a] - I[Net#a]) < 1;
+  assume I[Net#a] == I[Net#b];
+  assume I[Net#b] == I[Net#c];
+  assume I[Net#c] == I[Net#d];
+  assume I[Net#d] == I[Net#e];
   assume (I[Net#c] > 0) ==> (M[Net#c][0] == M[Net#a][0]);
   assume (I[Net#c] > 0) ==> (M[Net#c][I[Net#c] - 1] == M[Net#b][I[Net#b]]);
-  assume true && (forall idx$: int :: 
-    (I[Net#a] <= idx$) && (idx$ < C[Net#a]) ==> (0 <= M[Net#a][idx$])
-  );
-  assume (R[Net#a] == C[Net#c]) && (R[Net#b] == C[Net#c]);
+  assume 0 <= M[Net#a][I[Net#a]];
+  assume R[Net#a] == C[Net#c];
+  assume R[Net#b] == C[Net#c];
   assume (forall i: int :: 
     (0 <= i) && (i < C[Net#c]) ==> (M[Net#c][i] == (M[Net#a][i] + M[Net#b][i]))
   );
@@ -538,21 +492,23 @@ procedure Net#anon$4#input#in#10()
   assume (forall i: int :: 
     ((0 + 1) <= i) && (i < (C[Net#b] - 0)) ==> (M[Net#b][i] == M[Net#e][i - 1])
   );
-  assume (R[Net#c] == C[Net#d]) && (R[Net#c] == C[Net#e]);
+  assume R[Net#c] == C[Net#d];
+  assume R[Net#c] == C[Net#e];
   assume (forall i: int :: 
     (0 <= i) && (i < C[Net#d]) ==> (M[Net#d][i] == M[Net#c][i]) && (M[Net#e][i] == M[Net#c][i])
   );
   C[Net#a] := C[Net#a] + 1;
   assume 0 <= M[Net#a][I[Net#a]];
-  assert {:msg "34.15: Channel invariant might be falsified by network input (#38)"} (I[Net#a] == I[Net#b]) && (I[Net#b] == I[Net#c]) && (I[Net#c] == I[Net#d]) && (I[Net#d] == I[Net#e]);
-  assert {:msg "35.15: Channel invariant might be falsified by network input (#39)"} (I[Net#c] > 0) ==> (M[Net#c][0] == M[Net#a][0]);
-  assert {:msg "36.15: Channel invariant might be falsified by network input (#40)"} (I[Net#c] > 0) ==> (M[Net#c][I[Net#c] - 1] == M[Net#b][I[Net#b]]);
-  assert {:msg "Channel invariant might be falsified by network input (#41)"} true && (forall idx$: int :: 
-    (I[Net#a] <= idx$) && (idx$ < C[Net#a]) ==> (0 <= M[Net#a][idx$])
-  );
+  assert {:msg "34.15: Channel invariant might be falsified by network input (#43)"} I[Net#a] == I[Net#b];
+  assert {:msg "35.15: Channel invariant might be falsified by network input (#44)"} I[Net#b] == I[Net#c];
+  assert {:msg "36.15: Channel invariant might be falsified by network input (#45)"} I[Net#c] == I[Net#d];
+  assert {:msg "37.15: Channel invariant might be falsified by network input (#46)"} I[Net#d] == I[Net#e];
+  assert {:msg "38.15: Channel invariant might be falsified by network input (#47)"} (I[Net#c] > 0) ==> (M[Net#c][0] == M[Net#a][0]);
+  assert {:msg "39.15: Channel invariant might be falsified by network input (#48)"} (I[Net#c] > 0) ==> (M[Net#c][I[Net#c] - 1] == M[Net#b][I[Net#b]]);
+  assert {:msg "27.14: Channel invariant might be falsified by network input (#49)"} 0 <= M[Net#a][I[Net#a]];
 }
 procedure Net#anon$4#exit#11()
-  modifies C, R, M, I, St;
+  modifies C, R, M, I;
 {
   var Net#add: Actor;
   var Net#del: Actor;
@@ -580,13 +536,15 @@ procedure Net#anon$4#exit#11()
   assume 0 <= I[Net#e];
   assume I[Net#e] <= R[Net#e];
   assume R[Net#e] <= C[Net#e];
-  assume (I[Net#a] == I[Net#b]) && (I[Net#b] == I[Net#c]) && (I[Net#c] == I[Net#d]) && (I[Net#d] == I[Net#e]);
+  assume I[Net#a] == I[Net#b];
+  assume I[Net#b] == I[Net#c];
+  assume I[Net#c] == I[Net#d];
+  assume I[Net#d] == I[Net#e];
   assume (I[Net#c] > 0) ==> (M[Net#c][0] == M[Net#a][0]);
   assume (I[Net#c] > 0) ==> (M[Net#c][I[Net#c] - 1] == M[Net#b][I[Net#b]]);
-  assume true && (forall idx$: int :: 
-    (I[Net#a] <= idx$) && (idx$ < C[Net#a]) ==> (0 <= M[Net#a][idx$])
-  );
-  assume (R[Net#a] == C[Net#c]) && (R[Net#b] == C[Net#c]);
+  assume 0 <= M[Net#a][I[Net#a]];
+  assume R[Net#a] == C[Net#c];
+  assume R[Net#b] == C[Net#c];
   assume (forall i: int :: 
     (0 <= i) && (i < C[Net#c]) ==> (M[Net#c][i] == (M[Net#a][i] + M[Net#b][i]))
   );
@@ -595,7 +553,8 @@ procedure Net#anon$4#exit#11()
   assume (forall i: int :: 
     ((0 + 1) <= i) && (i < (C[Net#b] - 0)) ==> (M[Net#b][i] == M[Net#e][i - 1])
   );
-  assume (R[Net#c] == C[Net#d]) && (R[Net#c] == C[Net#e]);
+  assume R[Net#c] == C[Net#d];
+  assume R[Net#c] == C[Net#e];
   assume (forall i: int :: 
     (0 <= i) && (i < C[Net#d]) ==> (M[Net#d][i] == M[Net#c][i]) && (M[Net#e][i] == M[Net#c][i])
   );
@@ -604,20 +563,19 @@ procedure Net#anon$4#exit#11()
   assume !((1 <= (C[Net#a] - R[Net#a])) && (1 <= (C[Net#b] - R[Net#b])));
   assume !(1 <= (C[Net#e] - R[Net#e]));
   assume !(1 <= (C[Net#c] - R[Net#c]));
-  assert {:msg "28.13: Network action postcondition might not hold (#42)"} M[Net#d][0] == M[Net#a][0];
-  assert {:msg "29.13: Network action postcondition might not hold (#43)"} (I[Net#d] > 0) ==> (M[Net#d][I[Net#d]] == (M[Net#d][I[Net#d] - 1] + M[Net#a][I[Net#a]]));
+  assert {:msg "28.13: Network action postcondition might not hold (#50)"} M[Net#d][0] == M[Net#a][0];
+  assert {:msg "29.13: Network action postcondition might not hold (#51)"} (I[Net#d] > 0) ==> (M[Net#d][I[Net#d]] == (M[Net#d][I[Net#d] - 1] + M[Net#a][I[Net#a]]));
   R[Net#d] := R[Net#d] + 1;
   I := R;
-  assert {:msg "34.15: The network might not preserve the channel invariant (#44)"} (I[Net#a] == I[Net#b]) && (I[Net#b] == I[Net#c]) && (I[Net#c] == I[Net#d]) && (I[Net#d] == I[Net#e]);
-  assert {:msg "35.15: The network might not preserve the channel invariant (#45)"} (I[Net#c] > 0) ==> (M[Net#c][0] == M[Net#a][0]);
-  assert {:msg "36.15: The network might not preserve the channel invariant (#46)"} (I[Net#c] > 0) ==> (M[Net#c][I[Net#c] - 1] == M[Net#b][I[Net#b]]);
-  assert {:msg "The network might not preserve the channel invariant (#47)"} true && (forall idx$: int :: 
-    (I[Net#a] <= idx$) && (idx$ < C[Net#a]) ==> (0 <= M[Net#a][idx$])
-  );
-  C[Net#b] := C[Net#b] - 1;
-  assert {:msg "26.3: The network might leave unread tokens on channel a (#48)"} C[Net#a] == R[Net#a];
-  assert {:msg "26.3: The network might leave unread tokens on channel b (#49)"} C[Net#b] == R[Net#b];
-  assert {:msg "26.3: The network might leave unread tokens on channel c (#50)"} C[Net#c] == R[Net#c];
-  assert {:msg "26.3: The network might not produce the specified number of tokens on output out (#51)"} C[Net#d] == R[Net#d];
-  assert {:msg "26.3: The network might leave unread tokens on channel e (#52)"} C[Net#e] == R[Net#e];
+  assert {:msg "34.15: The network might not preserve the channel invariant (#52)"} I[Net#a] == I[Net#b];
+  assert {:msg "35.15: The network might not preserve the channel invariant (#53)"} I[Net#b] == I[Net#c];
+  assert {:msg "36.15: The network might not preserve the channel invariant (#54)"} I[Net#c] == I[Net#d];
+  assert {:msg "37.15: The network might not preserve the channel invariant (#55)"} I[Net#d] == I[Net#e];
+  assert {:msg "38.15: The network might not preserve the channel invariant (#56)"} (I[Net#c] > 0) ==> (M[Net#c][0] == M[Net#a][0]);
+  assert {:msg "39.15: The network might not preserve the channel invariant (#57)"} (I[Net#c] > 0) ==> (M[Net#c][I[Net#c] - 1] == M[Net#b][I[Net#b]]);
+  assert {:msg "32.13: The network might not preserve the network invariant (#58)"} (C[Net#b] - R[Net#b]) == 1;
+  assert {:msg "26.3: The network might leave unread tokens on channel a (#59)"} (C[Net#a] - R[Net#a]) == 0;
+  assert {:msg "26.3: The network might leave unread tokens on channel c (#60)"} (C[Net#c] - R[Net#c]) == 0;
+  assert {:msg "26.3: The network might not produce the specified number of tokens on output out (#61)"} (C[Net#d] - R[Net#d]) == 0;
+  assert {:msg "26.3: The network might leave unread tokens on channel e (#62)"} (C[Net#e] - R[Net#e]) == 0;
 }
